# Section 2.3: Q 7

Give the reason(s) for each step needed to show that the following argument is valid:

$[p \land (p \rightarrow q) \land (s \lor r) \land(r \rightarrow \lnot q)] \rightarrow (s \lor t)$

|#|__Steps__ | __Reasons__ |
|--| --| --|
|1|$p$ | |
|2|$p \rightarrow q$ | |
|3|$q$ | |
|4|$r \rightarrow \lnot q$ | |
|5|$q \rightarrow \lnot r$ | |
|6|$\lnot r$ | |
|7|$s \lor r$| |
|8|$s$ ||
|9|$\therefore (s\lor t)$| |

## Solution

Using rule of conjunction, $[p \land (p \rightarrow q) \land (s \lor r) \land(r \rightarrow \lnot q)] \rightarrow (s \lor t)$ can be rewritten as:

$p\\(p \rightarrow q)\\(s \lor r)\\(r \rightarrow \lnot q)]\\ \therefore s \lor t$
